Complete verification of Pkg

src/tls/DefineTable.fst
@@ -7,12 +7,67 @@ module DM = FStar.DependentMap
 module MH = FStar.Monotonic.Heap
 module HS = FStar.HyperStack
 
+open FStar.HyperStack.ST
+
 friend FStar.Monotonic.DependentMap
+
+let alloc #it vt =
+  if model then
+    MDM.alloc #it #vt #(fun _ -> True) #tls_define_region ()
+  else ()
+
+let extend #it #vt t i k =
+  if model then
+   begin
+    let t0 = ideal t in
+    recall t0;
+    t0 := MDM.upd !t0 i k;
+    mr_witness t0 (MDM.contains t0 i k)
+   end
+  else ()
 
 let dt_forall #it #vt t pred h =
   model ==> (forall (i:it) (k:vt i).
   {:pattern (defined_as t i k h)}
-  defined_as t i k h ==> pred i k h)
+  defined_as t i k h ==> pred k h)
+
+val fold_gtot: ('a -> 'b -> GTot 'a) -> 'a -> l:list 'b -> GTot 'a (decreases l)
+let rec fold_gtot f x l = match l with
+  | [] -> x
+  | hd::tl -> f (fold_gtot f x tl) hd
+
+let fp_add (#it:eqtype) (#vt:it->Type) (#p:M.loc) (fp:local_fp vt p)
+  (l:sub_loc p) (cur:(i:it & vt i)) : GTot (sub_loc p) =
+  let (| i, k |) = cur in
+  M.loc_union l (fp k)
+
+let footprint #it #vt t #parent fp h =
+  if model then 
+    let l = HS.sel h (ideal t) in
+    fold_gtot (fp_add fp) M.loc_none l
+  else M.loc_none
+
+let lemma_footprint_frame #it #vt t #p fp h0 h1 = ()
+
+let lemma_footprint_extend #it #vt t #p fp i k h0 h1 = ()
+
+let rec lemma_fp_includes (#it:eqtype) (vt:it->Type) (t:MDM.map it vt)
+  (#p:M.loc) (fp:local_fp vt p) (i:it) (k:vt i)
+  : Lemma (requires (MDM.sel t i == Some k))
+  (ensures fold_gtot (fp_add fp) M.loc_none t `M.loc_includes` (fp k))
+  (decreases %[t])
+  =
+  match t with
+  | [] -> ()
+  | (| x, y |) :: tl ->
+    if x = i then ()
+    else lemma_fp_includes vt tl fp i k
+
+let lemma_footprint_includes #it #vt t #p fp i k h =
+  if model then
+    let t0 = HS.sel h (ideal t) in
+    lemma_fp_includes vt t0 fp i k
+  else ()
 
 let lemma_forall_empty #it #vt t pred h = ()
 
@@ -23,39 +78,41 @@ val lemma_forall_extend_wit:
   #vt: (it -> Type) ->
   t: MDM.map it vt ->
   t': MDM.map it vt ->
-  pred: (i:it -> vt i -> mem -> GTot Type0) ->
-  i: it -> k: vt i ->
+  pred: (#i:it -> vt i -> mem -> GTot Type0) ->
+  #i: it -> k: vt i ->
   h: mem ->
   x:it -> y:vt x ->
   Lemma
-    (requires model /\ pred i k h /\
-      ((MDM.sel t x == Some y) ==> pred x y h) /\
+    (requires model /\ pred k h /\
+      ((MDM.sel t x == Some y) ==> pred #x y h) /\
       t' == (| i, k |) :: t)
-    (ensures (MDM.sel t' x == Some y) ==> pred x y h)
+    (ensures (MDM.sel t' x == Some y) ==> pred #x y h)
 
-let lemma_forall_extend_wit #it #vt t t' pred i k h x y = ()
+let lemma_forall_extend_wit #it #vt t t' pred #i k h x y = ()
 
-let lemma_forall_extend #it #vt t pred pred_frame i k h0 h1 =
+let lemma_forall_extend #it #vt t pred #p fp pred_frame #i k h0 h1 =
   if model then
     let t0 = HS.sel h0 (ideal t) in
     let t1 = HS.sel h1 (ideal t) in
-    let pred_frame' (i:it) (k:vt i) (h0:mem) (h1:mem)
-      : Lemma ((pred i k h0 /\ M.modifies (loc t) h0 h1) ==> pred i k h1) =
-      FStar.Classical.move_requires (pred_frame i k h0) h1
+    let pred_frame' (#i:it) (k:vt i) (h0:mem) (l:M.loc) (h1:mem)
+      : Lemma ((pred k h0 /\ M.modifies l h0 h1 /\
+        M.loc_disjoint l (fp k)) ==> pred k h1) =
+      FStar.Classical.move_requires (pred_frame k h0 l) h1
       in
-    let lupd (x:it) (y:vt x) : Lemma
-      (requires (MDM.sel t0 x == Some y) ==> pred x y h0)
-      (ensures (MDM.sel t1 x == Some y) ==> pred x y h1) =
+    let lupd (#x:it) (y:vt x) : Lemma
+      (requires (MDM.sel t0 x == Some y) ==> pred #x y h0)
+      (ensures (MDM.sel t1 x == Some y) ==> pred #x y h1) =
       assert(MDM.sel t1 x == (if x = i then Some k else MDM.sel t0 x));
       if x = i then ()
-      else pred_frame' x y h0 h1
+      else pred_frame' #x y h0 (loc t) h1
       in
     let prove_on_witness (x:it) (y:vt x)
-      : Lemma (MDM.sel t1 x == Some y ==> pred x y h1)
+      : Lemma (MDM.sel t1 x == Some y ==> pred #x y h1)
       =
       lemma_forall_elim t pred x y h0;
-      lupd x y;
-      lemma_forall_extend_wit t0 t1 pred i k h1 x y in
+      lupd #x y;
+      lemma_forall_extend_wit t0 t1 pred #i k h1 x y
+      in
     FStar.Classical.forall_intro_2 prove_on_witness
   else ()
 
@@ -63,46 +120,45 @@ val lemma_forall_frame_wit:
   #it: eqtype ->
   #vt: (it -> Type) ->
   t: dt vt ->
-  pred: (i:it -> vt i -> mem -> GTot Type0) ->
-  pred_fp: M.loc ->
-  pred_frame: (i:it -> k:vt i -> h0:mem -> l:M.loc -> h1:mem -> Lemma
-    ((pred i k h0 /\ M.modifies l h0 h1 /\ M.loc_disjoint l pred_fp)
-     ==> pred i k h1)) ->
+  pred: (#i:it -> vt i -> mem -> GTot Type0) ->
+  #parent: M.loc ->
+  fp: local_fp vt parent ->
+  pred_frame: (#i:it -> k:vt i -> h0:mem -> l:M.loc -> h1:mem -> Lemma
+    ((pred k h0 /\ M.modifies l h0 h1 /\ M.loc_disjoint l (fp k))
+     ==> pred k h1)) ->
   h0: mem -> l:M.loc -> h1: mem ->
   x:it -> y:vt x ->
   Lemma
-    (requires M.modifies l h0 h1 /\ t `used_in` h0 /\
-      (defined_as t x y h0 ==> pred x y h0) /\
-      M.loc_disjoint (loc t) l /\ M.loc_disjoint pred_fp l)
-    (ensures defined_as t x y h1 ==> pred x y h1)
+    (requires M.modifies l h0 h1 /\ t `live` h0 /\
+      (defined_as t x y h0 ==> pred y h0) /\
+      M.loc_disjoint l (loc t) /\ M.loc_disjoint l (fp y))
+    (ensures defined_as t x y h1 ==> pred y h1)
 
-let lemma_forall_frame_wit #it #vt t pred pred_fp pred_frame h0 l h1 x y =
-  lemma_frame_dt t h0 l h1;
-  pred_frame x y h0 l h1
+let lemma_forall_frame_wit #it #vt t pred #p fp pred_frame h0 l h1 x y =
+  lemma_unchanged_frame t h0 l h1;
+  pred_frame y h0 l h1
 
-let lemma_forall_frame #it #vt t pred pred_fp pred_frame h0 l h1 =
+// Could be simplified if FStar.Classical had
+// move_requires_2 or forall_impl_intro_2
+let lemma_forall_frame #it #vt t pred #p fp pred_frame h0 l h1 =
   if model then 
-    let pred_frame' (i:it) (k:vt i) (h0:mem) (l:M.loc) (h1:mem)
-      : Lemma ((pred i k h0 /\ M.modifies l h0 h1 /\ M.loc_disjoint l pred_fp)
-         ==> pred i k h1) =
-      FStar.Classical.move_requires (pred_frame i k h0 l) h1
+    let pred_frame' (#i:it) (k:vt i) (h0:mem) (l:M.loc) (h1:mem)
+      : Lemma ((pred k h0 /\ M.modifies l h0 h1 /\ M.loc_disjoint l (fp k))
+         ==> pred k h1) =
+      FStar.Classical.move_requires (pred_frame k h0 l) h1
       in
-    let prove_on_witness (x:it) (y:vt x)
-      : Lemma (defined_as t x y h1 ==> pred x y h1)
+    let prove_on_witness (v:(i:it & vt i))
+      : Lemma (requires defined_as t (dfst v) (dsnd v) h1)
+        (ensures pred (dsnd v) h1)
       =
+      let (| x, y |) = v in
       lemma_forall_elim t pred x y h0;
-      lemma_forall_frame_wit t pred pred_fp pred_frame' h0 l h1 x y in
-    FStar.Classical.forall_intro_2 prove_on_witness
+      lemma_footprint_includes t fp x y h0;
+      lemma_forall_frame_wit t pred fp pred_frame' h0 l h1 x y
+      in
+    let prove_on_witness2 (x:it) (y:vt x)
+      : Lemma (defined_as t x y h1 ==> pred y h1)
+      = FStar.Classical.move_requires prove_on_witness (|x,y|)
+      in
+    FStar.Classical.forall_intro_2 prove_on_witness2
   else ()
-
-val fold_gtot: ('a -> 'b -> GTot 'a) -> 'a -> l:list 'b -> GTot 'a (decreases l)
-let rec fold_gtot f x l = match l with
-  | [] -> x
-  | hd::tl -> fold_gtot f (f x hd) tl
-
-let footprint #it #vt t fp h =
-  if model then 
-    let l = HS.sel h (ideal t) in
-    fold_gtot (fun l (| i, k |) -> M.loc_union l (fp i k)) M.loc_none l
-  else M.loc_none
-
