src/tls/DefineTable.fsti
@@ -32,11 +32,23 @@ inline_for_extraction type dt (#it:eqtype) (vt:it->Type) =
 let ideal (#it:eqtype) (#vt:it->Type) (t:dt vt) : Pure (table vt)
   (requires model) (ensures fun _ -> True) = t
 
+let real (#it:eqtype) (#vt:it->Type) (t:dt vt) : Pure unit
+  (requires not model) (ensures fun _ -> True) = t
+
 let loc (#it:eqtype) (#vt:it->Type) (t:dt vt) =
-  if model then M.loc_mreference (ideal t) else M.loc_none
+  (if model then M.loc_mreference (ideal t) else M.loc_none)
+
+type live (#it:eqtype) (#vt:it -> Type) (t:dt vt) (h:mem) =
+  (model ==> h `HS.contains` (ideal t))
 
 type fresh (#it:eqtype) (#vt:it -> Type) (t:dt vt) (i:it) (h:mem) =
-  model ==> MDM.fresh (ideal t) i h
+  (model ==> MDM.fresh (ideal t) i h)
+
+let lemma_fresh_frame (#it:eqtype) (#vt:it -> Type) (t:dt vt) (i:it)
+  (h0:mem) (l:M.loc) (h1:mem) : Lemma
+  (requires fresh t i h0 /\ M.modifies l h0 h1 /\
+    M.loc_disjoint l (loc t) /\ live t h0)
+  (ensures fresh t i h1) = ()
 
 type defined_as (#it:eqtype) (#vt:it -> Type) (t:dt vt) (i:it) (k:vt i) (h:mem) =
   model ==> (MDM.sel (HS.sel h (ideal t)) i == Some k)
@@ -56,6 +68,11 @@ type extended (#it:eqtype) (#vt:it -> Type) (t:dt vt)
 type unchanged (#it:eqtype) (#vt:it -> Type) (t:dt vt) (h0 h1:mem) =
   model ==> HS.sel h0 (ideal t) == HS.sel h1 (ideal t)
 
+let lemma_unchanged_frame (#it:eqtype) (#vt:it -> Type) (t:dt vt)
+  (h0:mem) (l:M.loc) (h1:mem) : Lemma
+  (requires M.modifies l h0 h1 /\ live t h0 /\ M.loc_disjoint l (loc t))
+  (ensures unchanged t h0 h1) = ()
+
 type empty (#it:eqtype) (#vt:it -> Type) (t:dt vt) (h1:mem) =
   model ==> HS.sel h1 (ideal t) == MDM.empty
 
@@ -63,26 +80,29 @@ type disjoint (#it:eqtype) (#vt:it -> Type) (t:dt vt)
   (#it':eqtype) (#vt':it' -> Type) (t':dt vt') =
   M.loc_disjoint (loc t) (loc t')
 
-let alloc (#it:eqtype) (vt:it -> Type) : ST (dt vt)
-  (requires fun h0 -> True)
-  (ensures fun h0 t h1 -> M.modifies (loc t) h0 h1 /\ empty t h1)
-  =
-  if model then (MDM.alloc #it #vt #(fun _ -> True) #tls_define_region ())
-  else ()
-
-type used_in (#it:eqtype) (#vt:it -> Type) (t:dt vt) (h:mem) =
-  model ==> h `HS.contains` (ideal t)
-
 let lemma_disjoint_unchanged (#it:eqtype) (#vt:it -> Type) (t:dt vt)
   (#it':eqtype) (#vt':it' -> Type) (t':dt vt') (h0:mem) (h1:mem) : Lemma
-  (requires M.modifies (loc t) h0 h1 /\
-    disjoint t t' /\ used_in t h0 /\ used_in t' h0)
+  (requires M.modifies (loc t) h0 h1 /\ disjoint t t' /\
+    live t h0 /\ live t' h0)
   (ensures unchanged t' h0 h1) = ()
 
-let lemma_frame_dt (#it:eqtype) (#vt:it -> Type) (t:dt vt)
-  (h0:mem) (l:M.loc) (h1:mem) : Lemma
-  (requires M.modifies l h0 h1 /\ used_in t h0 /\ M.loc_disjoint l (loc t))
-  (ensures unchanged t h0 h1) = ()
+val alloc:
+  #it:eqtype ->
+  vt: (it -> Type) ->
+  ST (dt vt)
+  (requires fun h0 -> True)
+  (ensures fun h0 t h1 -> M.modifies M.loc_none h0 h1 /\
+    empty t h1 /\ fresh_loc (loc t) h0 h1)
+
+val extend:
+  #it:eqtype ->
+  #vt: (it -> Type) ->
+  t: dt vt ->
+  i: it ->
+  k: vt i ->
+  ST unit
+  (requires fun h0 -> fresh t i h0)
+  (ensures fun h0 () h1 -> extended t i k h0 h1)
 
 (* Used to define a joint invariant over all defined instances
 The definition is opaque but the lemmas below are enough to use
@@ -91,15 +111,67 @@ val dt_forall:
   #it: eqtype ->
   #vt: (it -> Type) ->
   t: dt vt ->
-  pred: (i:it -> vt i -> mem -> GTot Type0) ->
+  pred: (#i:it -> vt i -> mem -> GTot Type0) ->
   h: mem ->
   Type0
+
+type local_fp (#it:eqtype) (vt:it->Type) (parent:M.loc) =
+  #i:it -> vt i -> sub_loc parent
+
+// Package footprint = union of all instance footprints
+val footprint:
+  #it: eqtype ->
+  #vt: (it -> Type) ->
+  t: dt vt ->
+  #parent: M.loc ->
+  fp: local_fp vt parent ->
+  h: mem ->
+  GTot (sub_loc parent)
+
+val lemma_footprint_frame:
+  #it: eqtype ->
+  #vt: (it -> Type) ->
+  t: dt vt ->
+  #parent: M.loc ->
+  fp: local_fp vt parent ->
+  h0: mem ->
+  h1: mem ->
+  Lemma
+    (requires unchanged t h0 h1)
+    (ensures footprint t fp h0 == footprint t fp h1)
+
+val lemma_footprint_extend: 
+  #it: eqtype ->
+  #vt: (it -> Type) ->
+  t: dt vt ->
+  #parent: M.loc ->
+  fp: local_fp vt parent ->
+  i: it ->
+  k: vt i ->
+  h0: mem ->
+  h1: mem ->
+  Lemma
+    (requires extended t i k h0 h1)
+    (ensures footprint t fp h1 == M.loc_union (footprint t fp h0) (fp k))
+
+val lemma_footprint_includes:
+  #it: eqtype ->
+  #vt: (it -> Type) ->
+  t: dt vt ->
+  #parent: M.loc ->
+  fp: local_fp vt parent ->
+  i: it ->
+  k: vt i ->
+  h: mem ->
+  Lemma
+    (requires defined_as t i k h)
+    (ensures (footprint t fp h) `M.loc_includes` (fp k))
 
 val lemma_forall_empty:
   #it: eqtype ->
   #vt: (it -> Type) ->
   t: dt vt ->
-  pred: (i:it -> vt i -> mem -> GTot Type0) ->
+  pred: (#i:it -> vt i -> mem -> GTot Type0) ->
   h: mem ->
   Lemma 
     (requires empty t h)
@@ -109,77 +181,48 @@ val lemma_forall_elim:
   #it: eqtype ->
   #vt: (it -> Type) ->
   t: dt vt ->
-  pred: (i:it -> vt i -> mem -> GTot Type0) ->
+  pred: (#i:it -> vt i -> mem -> GTot Type0) ->
   i: it -> k: vt i ->
   h: mem ->
   Lemma
     (requires dt_forall t pred h /\ model)
-    (ensures defined_as t i k h ==> pred i k h)
+    (ensures defined_as t i k h ==> pred k h)
 
 val lemma_forall_extend:
   #it: eqtype ->
   #vt: (it -> Type) ->
   t: dt vt ->
-  pred: (i:it -> vt i -> mem -> GTot Type0) ->
-  pred_frame: (i:it -> k:vt i -> h0:mem -> h1:mem -> Lemma
-    (requires pred i k h0 /\ M.modifies (loc t) h0 h1)
-    (ensures pred i k h1)) ->
-  i: it -> k: vt i ->
+  pred: (#i:it -> vt i -> mem -> GTot Type0) ->
+  #parent: M.loc ->
+  fp: local_fp vt parent ->
+  pred_frame: (#i:it -> k:vt i -> h0:mem -> l:M.loc -> h1:mem -> Lemma
+    (requires pred k h0 /\ M.modifies l h0 h1 /\ M.loc_disjoint l (fp k))
+    (ensures pred k h1)) ->
+  #i: it -> k: vt i ->
   h0: mem -> h1: mem ->
   Lemma
-    (requires dt_forall t pred h0 /\
-      extended t i k h0 h1 /\ pred i k h1)
+    (requires dt_forall t pred h0 /\ extended t i k h0 h1 /\
+      pred k h1 /\ M.loc_disjoint (loc t) parent)
     (ensures dt_forall t pred h1)
 
 val lemma_forall_frame:
   #it: eqtype ->
   #vt: (it -> Type) ->
   t: dt vt ->
-  pred: (i:it -> vt i -> mem -> GTot Type0) ->
-  pred_fp: M.loc ->
-  pred_frame: (i:it -> k:vt i -> h0:mem -> l:M.loc -> h1:mem -> Lemma
-    (requires pred i k h0 /\ M.modifies l h0 h1 /\ M.loc_disjoint l pred_fp)
-    (ensures pred i k h1)) ->
+  pred: (#i:it -> vt i -> mem -> GTot Type0) ->
+  #parent: M.loc ->
+  fp: local_fp vt parent ->
+  pred_frame: (#i:it -> k:vt i -> h0:mem -> l:M.loc -> h1:mem -> Lemma
+    (requires pred k h0 /\ M.modifies l h0 h1 /\ M.loc_disjoint l (fp k))
+    (ensures pred k h1)) ->
   h0: mem -> l:M.loc -> h1: mem ->
   Lemma
     (requires dt_forall t pred h0
-      /\ M.modifies l h0 h1 /\ t `used_in` h0
-      /\ M.loc_disjoint (loc t) l /\ M.loc_disjoint pred_fp l)
+      /\ M.modifies l h0 h1 /\ t `live` h0
+      /\ M.loc_disjoint l (loc t) /\ M.loc_disjoint l (footprint t fp h0))
     (ensures dt_forall t pred h1)
 
-val footprint:
-  #it: eqtype ->
-  #vt: (it -> Type) ->
-  t: dt vt ->
-  fp: (i:it -> vt i -> M.loc) -> // Instance footprint
-  h: mem ->
-  GTot M.loc // Package footprint = union of all instance footprints
-
-val lemma_footprint_extend: 
-  #it: eqtype ->
-  #vt: (it -> Type) ->
-  t: dt vt ->
-  fp: (i:it -> vt i -> M.loc) ->
-  i: it ->
-  k: vt i ->
-  h0: mem ->
-  h1: mem ->
-  Lemma
-    (requires extended t i k h0 h1)
-    (ensures footprint t fp h1 == M.loc_union (footprint t fp h0) (fp i k))
-
-val lemma_footprint_includes:
-  #it: eqtype ->
-  #vt: (it -> Type) ->
-  t: dt vt ->
-  fp: (i:it -> vt i -> M.loc) ->
-  i: it ->
-  k: vt i ->
-  h: mem ->
-  Lemma
-    (requires defined_as t i k h)
-    (ensures (footprint t fp h) `M.loc_includes` (fp i k))
-
+(*
 val dt_fold:
   #it: eqtype ->
   #vt: (it -> Type) ->
@@ -189,3 +232,4 @@ val dt_fold:
   f: (rt -> i:it -> vt i -> rt) ->
   h: mem ->
   GTot rt
+*)
